coq/SigmaHCOL/SigmaHCOL.v
@@ -1111,22 +1111,9 @@ TODO: remove
     mkSHOperator Monoid_RthetaSafeFlags i o
                  (Diamond dot initial (get_family_op Monoid_RthetaSafeFlags op_family))
                  _
-                 (* !!! (IReduction_mem dot (get_family_mem_op _ op_family))
-                 _ *)
                  (family_in_index_set _ op_family)
                  (family_out_index_set _ op_family) (* All scatters must be the same but we do not enforce it here. However if they are the same, the union will equal to any of them, so it is legit to use union here *)
   .
-
-  (*
-
-  In SPIRAL [ISumReduction] is what we call [ISumReduction] and strictly speaking there is no equivalent to [ISumReduction] as defined below. [ISumReduction] defined below is basically row-wise sum. To avoid confusion we will not use [ISumReduction] name for now.
-
-  Definition ISumReduction
-             {i o n}
-             (op_family: @SHOperatorFamily Monoid_RthetaSafeFlags i o n)
-    :=
-      @IReduction i o n plus _ zero op_family.
-   *)
 
   Global Instance IReduction_proper
          {i o n: nat}
